\section{Lecture 3. Exponential model. Methods of point evaluation contruction}

Let $X_1, \ldots, X_n$ a sample from regular parametric model
$\mathcal{F} = \{F(x, \theta), \theta \in \Theta\} $ ;
$f(x, \theta)$ --- probability density function (or $P(X_1 = x)$ in
descrete variant).
$g(\theta)$ --- some differentiable parametric function;
$K_{0}^{g}$ --- class of unbiased evaluations for $g(\theta)$.

Then:
\begin{equation}
    \label{eq:3:effective-evaluation-equality}
    \forall T \in K_{0}^{g}: \mathcal{D}_{\theta} T \geq \frac{\left[ 
    g'(\theta)\right] ^2}{n\cdot i(\theta)}
\end{equation}
where
\[
i(\theta) = M_{\theta}\left( \frac{\partial}{\partial \theta} \ln f(x, \theta) \right) ^2
\] 
is quantity of Fisher information.
Besides:
\[
\mathcal{D}_{\theta} T = \frac{\left[ g'(\theta) \right] ^2}{n i(\theta)} \iff
T - g(\theta) = a(\theta) U(\vec{X}, \theta)
\] 
where  $U(\vec{X}, \theta) = \frac{\partial}{\partial \theta} \ln
\mathcal{L}(\vec{X}, \theta)$ --- sample contribution.

The statistics for which the equation \ref{eq:3:effective-evaluation-equality}
is true is called effective evaluation.



\subsection{Exponential model}

\begin{definition}
    Model $\mathcal{F} = \{F(x, \theta), \theta \in \Theta\} $ is called 
    exponential if function $f(x, \theta)$ is like:
    \[
        f(x, \theta) = \exp{A(\theta) \cdot B(x) + C(\theta) + D(x)}
    \] 
    or
    \[
    \ln f(x, \theta) = A(\theta) \cdot B(x) + C(\theta) + D(x)
    .\] 
\end{definition}

\begin{example}[$\operatorname{Bin}$ is exponential model]
    \[
    X_i \sim \operatorname{Bin}(k, \theta);
    \] 
    \begin{gather*}
        f(x, \theta) = P(X = x) = C_k^x \theta^x \left( 1 - \theta \right) ^{k-x}
        \quad x = \overline{0, k}
    \end{gather*}
    \begin{gather*}
        \ln f(x, \theta) = \ln C_k ^x + x \ln \theta + \left( k-x \right) 
        \ln(1- \theta) = \\
        = \underbrace{\ln k! + \ln \frac{1}{x! \left( k-x \right) !}}_{D(x)}
        + \underbrace{x\ln \frac{\theta}{1 - \theta}}_{B(x)\cdot A(\theta)}
        + \underbrace{k \ln(1 - \theta)}_{C(\theta)}
    \end{gather*}
    So model $\operatorname{Bin}(k, \theta)$ is exponential.
\end{example}
\begin{remark}
    Models $\mathcal{N}(\theta, \sigma^2)$, $\mathcal{N}(a, \theta^2)$,
    $\operatorname{Poiss}(\theta)$, $\Gamma(\theta, \lambda)$ are
    \textbf{exponential} models
\end{remark}

\begin{example}
    Causy distribution is not an exponential model.
    Indeed:
    \[
    f(x, \theta) = \frac{1}{\pi} \cdot \frac{1}{1 + \left( x - \theta
    \right) ^2}, \quad \theta\in \mathbb{R}, \; x \in \mathbb{R}
    .\] 
    \[
    \ln f(x, \theta) = C - \ln \left( 1 + \left( x - \theta \right) ^2 \right) 
    .\] 
    Assume that
    \[
    \ln f(x, \theta) = A(\theta) B(x) + C(\theta) + D(x)
    \] 
    then \[
        \frac{\partial ^2}{\partial \theta \partial x} \ln f(x, \theta) =
        A'(\theta) B'(x) \equiv a(\theta) b(x)
    .\] 
    On the other side:
    \[
    \frac{\partial ^2}{\partial \theta \partial x} \ln f(x, \theta) = 
    2 \cdot \frac{1 - (x- \theta)^2}{\left( 1 + (x- \theta)^2 \right) ^2}
    .\] 
    Therefore:
    \[
    a(\theta) \cdot b(x) = 2 \cdot \frac{1 - (x- \theta)^2}{\left(
    1 + (x - \theta)^2 \right) ^2}
    .\] 
    But the right side cannot be represented as $a(\theta) b(x)$
    (separate the variables).
\end{example}


Lets compute sample contribution for a regular exponential
model:
\begin{gather*}
    U(\vec{X}, \theta) = \frac{\partial }{\partial \theta} \ln
    \mathcal{L}(\vec{X}, \theta) = \\
    = \frac{\partial }{\partial \theta} \ln \prod_{i=1}^{n} 
    \exp{A(\theta)B(X_i) + C(\theta) + D(X_i)} = \\
    = \frac{\partial }{\partial \theta} \ln
    \exp{A(\theta) \cdot \sum_{i=1}^{n} B(X_i) + n C(\theta) + \sum_{i=1}^{n} D(X_i)} = \\
    = \frac{\partial }{\partial \theta} \left( A(\theta)
    \cdot n \cdot \overline{B(X)} + n C(\theta) + \overline{D(X)} \cdot n\right) = \\ 
    = A'(\theta)  \cdot n \cdot \overline{B(X)} + n \cdot C'(\theta) = 
    n A'(\theta) \left[ \overline{B(X)} + \frac{C'(\theta)}{A'(\theta)} \right] 
\end{gather*}
where $\overline{B(X)} = \frac{1}{n} \sum_{i=1}^{n} B(X_i)$.
Suppose:
\[
a(\theta) = \frac{1}{n A'(\theta)} \quad T(\vec{X}) = \overline{B(x)}
\quad g(\theta) = - \frac{C'(\theta)}{A'(\theta)}
.\] 
then:
\[
 T(x) - g(\theta) = a(\theta) \cdot U(\vec{X}, \theta)
.\] 
By Cramer-Rao criterion: $T(x) = \overline{B(x)}$ is an effective evaluation
for $g(\theta) = - \displaymath \frac{C'(\theta)}{A'(\theta)}$.
